We first prove the following lemma.
\begin{lemma}
\label{lemcoding}
For each $T=1, 2, ...$, we have
\[
I(\bar{X}^{T} \rightarrow W^{T} || U^{T-1},\tilde{X}^{T}) \geq I(\bar{X}^{T} \rightarrow U^{T} || \tilde{X}^{T}).
\]
\end{lemma}
\begin{proof}
The result is established by the following chain of inequalities.
\begin{align*}
&  I(\bar{X}^T \rightarrow W^T || U^{T-1},\tilde{X}^T) - I(\bar{X}^T \rightarrow U^T || \tilde{X}^T)  \\
& = \sum_{t=0}^T I\left(\bar{X}^t;W_t|W^{t-1},U^{t-1},\tilde{X}^t \right) - I\left(\bar{X}^t;U_t|U^{t-1},\tilde{X}^t \right)\\
& \stackrel{\text{(a)}}{=} \sum_{t=0}^T I\left(\bar{X}^t;W_t,U_t|W^{t-1},U^{t-1},\tilde{X}^t \right) \\
& \hspace{10ex}- I\left(\bar{X}^t;U_t|U^{t-1},\tilde{X}^t \right)\\
& \stackrel{\text{(b)}}{=} \sum_{t=0}^T I\left(\bar{X}^t;W^t|U^{t},\tilde{X}^t \right) - I\left(\bar{X}^t;W^{t-1}|U^{t-1},\tilde{X}^t \right)\\
& \stackrel{\text{(c)}}{=} \sum_{t=0}^T I\left(\bar{X}^t;W^t|U^{t},\tilde{X}^t \right) - I\left(\bar{X}^{t-1};W^{t-1}|U^{t-1},\tilde{X}^t \right)\\
& \stackrel{\text{(d)}}{\geq} \sum_{t=0}^T I\left(\bar{X}^t;W^t|U^{t},\tilde{X}^t \right) - I\left(\bar{X}^{t-1};W^{t-1}|U^{t-1},\tilde{X}^{t-1} \right)\\
& \stackrel{\text{(e)}}{=} I\left(\bar{X}^T;W^T | U^T,\tilde{X}^T \right) \geq 0. 
\end{align*}
Equality (a) holds since
\begin{align*}
&I(\bar{X}^t; W_t, U_t|W^{t-1}, U^{t-1}, \tilde{X}^t)=\\
&I(\bar{X}^t; W_t|W^{t-1}, U^{t-1}, \tilde{X}^t)
+I(\bar{X}^t; U_t|W^t, U^{t-1}, \tilde{X}^t)
\end{align*}
and the second term is zero since $U_t$ is conditionally independent of $\bar{X}^t$ given $(W^t, U^{t-1})$. Equality (b) can be shown by applying the chain rule for mutual information in two different ways:
\begin{align*}
&I(\bar{X}^t; W^t, U_t|U^{t-1}, \tilde{X}^t) \\
&=I(\bar{X}^t; W^{t-1}|U^{t-1}, \tilde{X}^t)+I(\bar{X}^t; W_t, U_t| W^{t-1}, U^{t-1}, \tilde{X}^t) \\
&=I(\bar{X}^t; U_t|U^{t-1}, \tilde{X}^t)+I(\bar{X}^t;W^t|U^t, \tilde{X}^t).
\end{align*}
Equality (c) holds since
\begin{align*}
&I(\bar{X}^t; W^{t-1}|U^{t-1}, \tilde{X}^t)=\\
&I(\bar{X}^{t-1}; W^{t-1}|U^{t-1}, \tilde{X}^t)+I(\bar{X}_t; W^{t-1}|U^{t-1}, \tilde{X}^t, \bar{X}^{t-1})
\end{align*}
and the second term is zero. To see (d), apply the chain rule in two different ways:
\begin{align*}
&I(\bar{X}^{t-1}, \tilde{X}_t; W^{t-1}|U^{t-1},\tilde{X}^{t-1}) \\
&=I(\tilde{X}_t; W^{t-1}|U^{t-1}, \tilde{X}^{t-1})+I(\bar{X}^{t-1}; W^{t-1}|U^{t-1}, \tilde{X}^t) \\
&=I(\bar{X}^{t-1}; W^{t-1}|U^{t-1}, \tilde{X}^{t-1}) \\
&\hspace{5ex}+I(\tilde{X}_t;W^{t-1}|U^{t-1},\tilde{X}^{t-1}, \bar{X}^{t-1}).
\end{align*}
Since the last term is zero, we have 
\[
I(\bar{X}^{t-1}; W^{t-1}|U^{t-1}, \tilde{X}^{t-1}) \geq I(\bar{X}^{t-1}; W^{t-1}|U^{t-1}, \tilde{X}^t).
\]
Finally, (e) is due to the telescopic cancellation.
\end{proof}

Theorem~\ref{theorate} can now be shown as
\begin{align*}
R&=\sum_{t=0}^{T-1} R_t \\
&\stackrel{\text{(a)}}{\geq} \sum\nolimits_{t=0}^{T-1} H(W_t) \\
&\stackrel{\text{(b)}}{\geq} \sum\nolimits_{t=0}^{T-1} H(W_t|W^{t-1}, U^{t-1}, \tilde{X}^t) \\
&\stackrel{\text{(c)}}{\geq} \sum\nolimits_{t=0}^{T-1} H(W_t|W^{t-1}, U^{t-1}, \tilde{X}^t) \\
&\hspace{10ex}-H(W_t|\bar{X}^t, W^{t-1}, U^{t-1}, \tilde{X}^t) \\
&=\sum\nolimits_{t=0}^{T-1} I(\bar{X}^t; W_t|W^{t-1}, U^{t-1}, \tilde{X}^t) \\
&=I(\bar{X}^{T-1}\rightarrow W^{T-1}\| U^{T-2}, \tilde{X}^{T-1}) \\
&\stackrel{\text{(d)}}{\geq} I(\bar{X}^{T-1}\rightarrow U^{T-1}\| \tilde{X}^{T-1})
\end{align*}
Inequality (a) is a standard result - Theorem 2.6.4 in \cite{cover2012elements}. Inequality (b) holds since conditioning does not increase entropy, and (c) is because entropy is non-negative. Finally, (d) is due to Lemma~\ref{lemcoding}.

